Let 
\begin{align}
	\vec{a} = \myvec{1\\1\\1} , \vec{b} = \myvec{2\\ -7 \\ 3}, 
\vec{c} = \myvec{\dfrac{1}{\sqrt{3}}\\[2ex] \dfrac{1}{\sqrt{3}} \\[2ex] -\dfrac{1}{\sqrt{3}}} 
\label{eq:chapters/12/10/2/1/1}
\end{align}
Then
\begin{align}
	\norm{\vec{a}}&=\sqrt{\vec{a}^{\top}\vec{a}}=\sqrt{3}, 
	\label{eq:chapters/12/10/2/1/3}
	\\ \norm{\vec{b}}&=\sqrt{\vec{b}^{\top}\vec{b}}= \sqrt{62}, 
	\label{eq:chapters/12/10/2/1/4}
	\\ \norm{\vec{c}}&=\sqrt{\vec{c}^{\top}\vec{c}}	
=1
	\label{eq:chapters/12/10/2/1/5}
\end{align}



