\begin{align}
	\overrightarrow{AB}+\overrightarrow{BC}+\overrightarrow{CA} &=
\vec{B}-\vec{A} + \vec{C} - \vec{B} + \vec{A} - \vec{C}
= 0
\\
	\overrightarrow{AB}+\overrightarrow{BC}-\overrightarrow{AC} &=
\vec{B}-\vec{A} + \vec{C} - \vec{B} - (\vec{C} - \vec{A})
= 0
\\
	\overrightarrow{AB}+\overrightarrow{BC}+\overrightarrow{AC} &=
\vec{B}-\vec{A} + \vec{C} - \vec{B} + \vec{C} - \vec{A}
= 2(\vec{C}-\vec{A})
\\
	\overrightarrow{AB}-\overrightarrow{CB}+\overrightarrow{CA} &=
\vec{B}-\vec{A} - (\vec{B} - \vec{C}) + \vec{A} - \vec{C}
= 0
\end{align}
