\begin{enumerate}[label=\thesubsection.\arabic*.,ref=\thesubsection.\theenumi]
	\item Perform the eigendecompositions 
    \begin{align}
	    \vec{MM}^\top &= \vec{U}\vec{D}_1\vec{U}^\top \label{eq:chapters/12/11/2/16/svd/decomp-1} \\
	    \vec{M}^\top\vec{M} &= \vec{V}\vec{D}_2\vec{V}^\top \label{eq:chapters/12/11/2/16/svd/decomp-2}
    \end{align}
	\item    The following expression is known as {\em singular value decomposition}
    \begin{align}
        \vec{M} = 
	\vec{U}\vec{\Sigma}\vec{V}^\top
        \label{eq:chapters/12/11/2/16/svd/M-svd}
    \end{align}
    where $\vec{\Sigma}$ is diagonal with
    entries obtained as in 
        \eqref{eq:chapters/12/11/2/16/svd/svd-params}.
 Substituting in 
        \eqref{eq:chapters/12/11/2/16/lsq/vec-eqn},
	\begin{align}
\vec{V}\vec{\Sigma}\vec{U}^\top\vec{U}\vec{\Sigma}\vec{V}^\top\bm{\kappa} &= \vec{V}\vec{\Sigma}\vec{U}^\top\brak{\vec{B}-\vec{A}} \\
\implies \vec{V}\vec{\Sigma}^2\vec{V}^\top\bm{\kappa} &= \vec{V}\vec{\Sigma}\vec{U}^\top\brak{\vec{B}-\vec{A}} \\
\implies \bm{\kappa} &= \brak{\vec{V}\vec{\Sigma}^2\vec{V}^\top}^{-1}\vec{V}\vec{\Sigma}\vec{U}^\top\brak{\vec{B}-\vec{A}} \\
\implies \bm{\kappa} &= \vec{V}\vec{\Sigma}^{-2}\vec{V}^\top\vec{V}\vec{\Sigma}\vec{U}^\top\brak{\vec{B}-\vec{A}} \\
\implies \bm{\kappa} &= \vec{V}\vec{\Sigma}^{-1}\vec{U}^\top\brak{\vec{B}-\vec{A}}
\label{eq:chapters/12/11/2/16/svd/kappa-sol}
\end{align}
    where $\vec{\Sigma}^{-1}$ is obtained by inverting the nonzero elements of
    $\vec{\Sigma}$. 
		\item 
	    From \eqref{eq:chapters/12/11/2/16/lsq/x1x2}, 
\begin{align}
	\vec{x}_1-\vec{x}_2 &= 
	\vec{A}+ \kappa_1\vec{m_1}
	 -\vec{B}  - \kappa_2\vec{m_2} 
	 \\
	 &=
	\vec{A} 
	 -\vec{B}  + \vec{M} 
	\bm{\kappa}
\end{align}
which, upon substitution from 
        \eqref{eq:chapters/12/11/2/16/svd/M-svd}
	yields
\begin{align}
	\vec{x}_1-\vec{x}_2 &= 
	\vec{A} 
	 -\vec{B}  + 
\vec{U}\vec{\Sigma}\vec{V}^\top
\vec{V}\vec{\Sigma}^{-1}\vec{U}^\top\brak{\vec{B}-\vec{A}}
\\
	&=
	\brak{	\vec{A} 
	 -\vec{B}}  \brak{\vec{I}- 
\vec{U}\vec{\Sigma}
	\vec{\Sigma}^{-1}\vec{U}^\top}
\end{align}
			Thus, 
    \begin{align}
	    \norm{\vec{x}_1-\vec{x}_2} = 
	\norm{\brak{	\vec{A} 
	 -\vec{B}}  \brak{\vec{I}- 
\vec{U}\vec{\Sigma}
	    \vec{\Sigma}^{-1}\vec{U}^\top}}
        \label{eq:chapters/12/11/2/16/svd/min-sol}
    \end{align}
\end{enumerate}
